src/PlutusIR/Semantics/Dynamic/Values.v
@@ -9,16 +9,17 @@ From Coq Require Import
   Arith.PeanoNat
   Program.Equality
 .
+Import ListNotations.
 Import PeanoNat.Nat.
 
 Inductive is_error : term -> Prop :=
   | IsError : forall T,
       is_error (Error T).
 
-Fixpoint arg_count (t : term) : nat :=
+Fixpoint args_len (t : term) : nat :=
   match t with
-  | Apply s t => 1 + arg_count s
-  | TyInst t T => 1 + arg_count t
+  | Apply s t => 1 + args_len s
+  | TyInst t T => 1 + args_len t
   | _ => 0
   end
 .
@@ -37,7 +38,7 @@ Inductive value : term -> Prop :=
       Forall value vs ->
       value (Constr T i vs)
   | V_AppliedBuiltin : forall f t,
-      arg_count t < arity f ->
+      args_len t < arity f ->
       applied f t ->
       value t
 
@@ -55,7 +56,8 @@ with applied : DefaultFun -> term -> Prop :=
 
 #[export] Hint Constructors value applied : core.
 
-Section value_ind.
+Section MULTIND.
+
 Context
   (P : term -> Prop)
   (Q : DefaultFun -> term -> Prop)
@@ -66,7 +68,7 @@ Context
   (H_IWrap : forall (F T : ty) (v : term), value v -> P v -> P (IWrap F T v))
   (H_Constant : forall c : constant, P (Constant c))
   (H_Constr : forall (T : ty) (i : nat) (vs : list term), Forall value vs -> Forall P vs -> P (Constr T i vs))
-  (H_AppliedBuiltin : forall f t, arg_count t < arity f -> applied f t -> Q f t -> P t)
+  (H_AppliedBuiltin : forall f t, args_len t < arity f -> applied f t -> Q f t -> P t)
 
   (H_Builtin : forall f, Q f (Builtin f))
   (H_Apply : forall f t v, value v -> P v -> applied f t -> Q f t -> Q f (Apply t v))
@@ -79,88 +81,56 @@ Fixpoint values__ind (H_value : forall (t : term), value t -> P t) (ts : list te
     | @Forall_cons _ _ x xs vx vxs => @Forall_cons _ _ x xs (H_value x vx) (values__ind H_value xs vxs)
   end.
 
-Fixpoint value__ind (t : term) (v : value t) {struct v} : P t :=
+Fixpoint value__multind (t : term) (v : value t) {struct v} : P t :=
   match v in (value t0) return (P t0) with
   | V_LamAbs x T t0 => H_LamAbs x T t0
   | V_TyAbs X K t0 => H_TyAbs X K t0
-  | V_IWrap F1 T v0 v1 => H_IWrap F1 T v0 v1 (value__ind v0 v1)
+  | V_IWrap F1 T v0 v1 => H_IWrap F1 T v0 v1 (value__multind v0 v1)
   | V_Constant u => H_Constant u
   | V_Constr T i ts vs => H_Constr T i ts vs
       ((fix F ts vs := match vs as vs in Forall _ ts return Forall P ts with
         | Forall_nil _ => Forall_nil _
-        | @Forall_cons _ _ t ts vt vts => @Forall_cons _ _ t ts (value__ind t vt) (F ts vts)
+        | @Forall_cons _ _ t ts vt vts => @Forall_cons _ _ t ts (value__multind t vt) (F ts vts)
       end) ts vs)
   | V_AppliedBuiltin f t H_arity app => H_AppliedBuiltin f t H_arity app (applied__ind f t app)
   end
 with applied__ind f t (H_a : applied f t) {struct H_a} : Q f t :=
   match H_a in (applied f0 t0) return (Q f0 t0) with
   | A_Builtin f => H_Builtin f
-  | A_Apply f t v H_val H_a => H_Apply f t v H_val (value__ind v H_val) H_a (applied__ind f t H_a)
+  | A_Apply f t v H_val H_a => H_Apply f t v H_val (value__multind v H_val) H_a (applied__ind f t H_a)
   | A_TyInst f t T H_a => H_TyInst f t T H_a (applied__ind f t H_a)
   end
 .
 
-End value_ind.
 
-Inductive result' : term -> Prop :=
-  | R'_Value t : value t -> result' t
-  | R'_Error T : result' (Error T)
-.
 
-(* Results represent the result of computation, which include values and errors *)
+End MULTIND.
+
 Inductive result : term -> Prop :=
-  | R_LamAbs : forall x T t0,
-      result (LamAbs x T t0)
-  | R_TyAbs : forall X K t,
-      result (TyAbs X K t)
-  | R_IWrap : forall F T v,
-      result v ->
-      ~ is_error v ->
-      result (IWrap F T v)
-  | R_Constant : forall u,
-      result (Constant u)
-  | R_Error : forall T,
-      result (Error T)
-  | R_Constr : forall T i vs,
-      Forall result vs ->
-      result (Constr T i vs)
-  .
+  | R_Value t : value t -> result t
+  | R_Error T : result (Error T)
+.
 
 #[export] Hint Constructors result : core.
 
-Section result_ind.
-Context
-  (P : term -> Prop)
-.
-Context
-  (H_LamAbs : forall (x : String.string) (T : ty) (t0 : term), P (LamAbs x T t0))
-  (H_TyAbs : forall (X : String.string) (K : kind) (t : term), P (TyAbs X K t))
-  (H_IWrap : forall (F T : ty) (v : term), result v -> P v -> ~ is_error v -> P (IWrap F T v))
-  (H_Constant : forall c : constant, P (Constant c))
-  (H_Error : forall T : ty, P (Error T))
-  (H_Constr : forall (T : ty) (i : nat) (vs : list term), Forall result vs -> Forall P vs -> P (Constr T i vs))
-.
-Fixpoint results__ind (H_result : forall (t : term), result t -> P t) (ts : list term) (vs : Forall result ts): Forall P ts :=
-  match vs as vs in Forall _ ts return Forall P ts with
-    | Forall_nil _ => Forall_nil _
-    | @Forall_cons _ _ x xs vx vxs => @Forall_cons _ _ x xs (H_result x vx) (results__ind H_result xs vxs)
-  end.
-Fixpoint result__ind (t : term) (v : result t) {struct v} : P t :=
-  match v in (result t0) return (P t0) with
-  | R_LamAbs x T t0 => H_LamAbs x T t0
-  | R_TyAbs X K t0 => H_TyAbs X K t0
-  | R_IWrap F1 T v0 v1 n => H_IWrap F1 T v0 v1 (result__ind v0 v1) n
-  | R_Constant u => H_Constant u
-  | R_Error T => H_Error T
-  | R_Constr T i ts vs => H_Constr T i ts vs
-      ((fix F ts vs := match vs as vs in Forall _ ts return Forall P ts with
-        | Forall_nil _ => Forall_nil _
-        | @Forall_cons _ _ t ts vt vts => @Forall_cons _ _ t ts (result__ind t vt) (F ts vts)
-      end) ts vs)
-  end
-.
+Lemma value__IWrap F T v : value v -> value (IWrap F T v).
+Admitted.
 
-End result_ind.
+Lemma result__IWrap F T r : result r <-> result (IWrap F T r).
+Admitted.
+
+Lemma result__Constr_cons T i r rs : result r /\ result (Constr T i rs) -> result (Constr T i (r :: rs)).
+Admitted.
+
+Lemma result__TyInst f v T : applied f v -> applied f (TyInst v T).
+Admitted.
+
+#[export] Hint Resolve
+  value__IWrap
+  result__IWrap
+  result__Constr_cons
+  result__TyInst
+  : core.
 
 
 Lemma value__is_error v : value v -> ~ is_error v.
@@ -173,16 +143,15 @@ Proof.
   inversion H1.
 Qed.
 
-Lemma value__result' v : value v -> result' v.
-Proof. auto using result'. Qed.
+#[export] Hint Resolve
+  value__is_error
+  : core.
+
 
 Lemma value__result v : value v -> result v.
-Admitted.
+Proof. auto using result. Qed.
 
-Lemma result'__value v : result' v -> ~ is_error v -> value v.
-Admitted.
-
-Lemma result__value v : result v -> ~ is_error v-> value v.
+Lemma result__value v : result v -> ~ is_error v -> value v.
 Admitted.
 
 Lemma is_error_dec t : {is_error t} + {~ is_error t}.
@@ -206,9 +175,10 @@ Defined.
 Lemma value_dec t : {value t} + {~ value t}.
 Admitted.
 
-Lemma result'_dec t : {result' t} + {~ result' t}.
+Lemma result_dec t : {result t} + {~ result t}.
 Admitted.
 
+(*
 Lemma result_dec t : {result t} + {~ result t}.
 Proof.
   apply term__rect with
@@ -231,7 +201,7 @@ Proof.
     + left. auto.
     + right. inversion 1. contradiction .
 Defined.
-
+*)
 
 
 Definition is_error_beq (t : term) : bool :=
@@ -243,25 +213,13 @@ Definition is_error_beq (t : term) : bool :=
 Fixpoint value_beq (t : term) : bool.
 Admitted.
 
-Fixpoint result'_beq (t : term) : bool.
+Fixpoint result_beq (t : term) : bool.
 Admitted.
-
-Fixpoint result_beq (t : term) :=
-  match t with
-    | LamAbs x T t0 => true
-    | TyAbs X K t   => true
-    | IWrap F T v   => result_beq v && negb (is_error_beq v)
-    | Constant u    => true
-    | Error T       => true
-    | _ => false
-  end
-  .
 
 Lemma value_beq__value : forall t, value_beq t = true <-> value t.
 Admitted.
-Lemma result'_dec__result' : forall t, result'_beq t = true <-> result' t.
+
+Lemma result_dec__result : forall t, result_beq t = true <-> result t.
 Admitted.
 
-Lemma dec_result_result : forall t, result_beq t = true -> result t.
-Admitted.
 
