src/PlutusIR/Semantics/Dynamic/Bigstep/EvalToValue.v
@@ -4,7 +4,6 @@ Require Import PlutusCert.PlutusIR.Semantics.Dynamic.Bigstep.
 
 
 Lemma compute_defaultfun__result : forall t v,
-    fully_applied t ->
     compute_defaultfun t = Datatypes.Some v ->
     result v.
 Proof with (try discriminate).
@@ -55,18 +54,6 @@ Proof with (try discriminate).
 Admitted.
 
 
-Lemma compute_defaultfun__result' : forall t v,
-    fully_applied t ->
-    compute_defaultfun t = Datatypes.Some v ->
-    result' v.
-Admitted.
-
-
-Lemma eval_builtin_partial__result :
-  forall t r, t =η=> r -> result r
-.
-Admitted.
-
 Lemma eval_to_result :
     (forall t v k, t =[k]=> v -> result v) /\
     (forall t v k, t =[k]=>nr v -> result v) /\
@@ -74,54 +61,23 @@ Lemma eval_to_result :
 Proof with (eauto with hintdb__eval_no_error).
   apply eval__multind.
   all: intros.
-  all: eauto using compute_defaultfun__result...
-  - (* E_IWrap *)
-    inversion H0...
-  - (* Constr*)
-    inversion H2.
-    + apply R_Constr.
-      constructor...
-  - (* Builtin Apply Partial *)
-    eauto using eval_builtin_partial__result. 
-  - (* Builtin TyInst Partial*)
-    eauto using eval_builtin_partial__result. 
-  - (* Builtin TyInst Partial*)
-    eauto using eval_builtin_partial__result. 
+  all: try (solve [eauto using
+    result__value, compute_defaultfun__result]).
+  - (* E_Unwrap *)
+    apply <- result__IWrap...
 Qed.
-
-Lemma eval_to_result' :
-    (forall t v k, t =[k]=> v -> result' v) /\
-    (forall t v k, t =[k]=>nr v -> result' v) /\
-    (forall bs0 t v k, t =[k]=>r v WITH bs0 -> result' v).
-Admitted.
 
 Corollary eval_to_result__eval : forall t v k,
     t =[k]=> v ->
     result v.
 Proof. apply eval_to_result. Qed.
 
-Corollary eval_to_result'__eval : forall t v k,
-    t =[k]=> v ->
-    result' v.
-Proof. apply eval_to_result'. Qed.
-
 Corollary eval_to_result__eval_bindings_nonrec : forall t v k,
     t =[k]=>nr v ->
     result v.
 Proof. apply eval_to_result. Qed.
 
-
-Corollary eval_to_result'__eval_bindings_nonrec : forall t v k,
-    t =[k]=>nr v ->
-    result' v.
-Proof. apply eval_to_result'. Qed.
-
 Corollary eval_to_result__eval_bindings_rec : forall bs0 t v k,
     t =[k]=>r v WITH bs0 ->
     result v.
 Proof. apply eval_to_result. Qed.
-
-Corollary eval_to_result'__eval_bindings_rec : forall bs0 t v k,
-    t =[k]=>r v WITH bs0 ->
-    result' v.
-Proof. apply eval_to_result'. Qed.
