src/PlutusIR/Semantics/Dynamic/Bigstep/EvalValue.v
@@ -2,31 +2,49 @@ Require Import PlutusCert.PlutusIR.
 
 Require Import PlutusCert.PlutusIR.Semantics.Dynamic.Bigstep.
 
+Require Import Lists.List.
 Require Import Lia.
+
+
+Definition Q f t :=
+  args_len t < arity f ->
+  t =[0]=> t
+.
+
+Lemma eval_value__Constr T i vs :
+  Forall value vs ->
+  Forall (fun t => t =[ 0 ]=> t) vs ->
+  Constr T i vs =[ 0 ]=> Constr T i vs
+.
+Proof.
+Admitted.
+
+Lemma eval_value :
+  forall v, value v -> v =[0]=> v.
+Proof with (autounfold; (eauto || (try lia))).
+  apply value__multind with (Q := Q).
+  all: intros.
+  all: try solve [constructor; eauto].
+  - auto using eval_value__Constr.
+  - unfold Q in *. auto.
+  - (* Apply *)
+    unfold Q in *.
+    intros H_arity.
+    assert (split : 0 = 0 + 0) by auto.
+    rewrite split.
+    eapply E_Apply_Builtin_Partial...
+    apply H2. unfold args_len in *; lia.
+  - (* TyInst *)
+    unfold Q in *.
+    intros H_arity.
+    eapply E_TyInst_Builtin_Partial...
+    unfold args_len in *.
+    apply H0; lia.
+Qed.
 
 Lemma eval_result :
   forall v, result v -> v =[0]=> v.
-Proof with (autounfold; (eauto || (try lia))).
-  apply result__ind.
-  all: intros.
-  all: try solve [constructor; eauto].
-  (* Constr*)
-  - induction vs.
-    + constructor.
-    + inversion H. inversion H0. subst.
-      eapply E_Constr_cons with (k_t := 0) (k_ts := 0)...
+Proof.
+  intros v r.
+  destruct r; eauto using eval, eval_value.
 Qed.
-
-Lemma eval_result' :
-  forall v, result' v -> v =[0]=> v.
-Admitted.
-
-Corollary eval_result__result : forall v,
-    result v ->
-    v =[0]=> v.
-Proof. apply eval_result. Qed.
-
-Corollary eval_result'__result' : forall v,
-    result' v ->
-    v =[0]=> v.
-Admitted.
